work on MemSemantics

NLustre/MemSemantics.v
@@ -58,7 +58,7 @@ Module Type MEMSEMANTICS
        (Import OpAux : OPERATORS_AUX   Op)
        (Import Clks  : CLOCKS      Ids)
        (Import Syn   : NLSYNTAX    Ids Op       Clks)
-       (Import Str   : STREAM          Op)
+       (Import Str   : STREAM             Op OpAux)
        (Import Ord   : ORDERED     Ids Op       Clks Syn)
        (Import Mem   : MEMORIES    Ids Op       Clks Syn)
        (Import IsF   : ISFREE      Ids Op       Clks Syn)
@@ -70,60 +70,74 @@ Module Type MEMSEMANTICS
 
   Definition memory := memory (stream val).
 
+  Definition mfby (ls: stream value) (ms: stream val) (xs: stream value) : Prop :=
+    forall n, match ls n with
+         | absent    => ms (S n) = ms n /\ xs n = absent
+         | present v => ms (S n) = v    /\ xs n = present (ms n)
+         end.
+
   Implicit Type M : memory.
 
-  Inductive msem_equation G :
-    stream bool -> stream bool -> history -> memory -> equation -> Prop :=
-  | SEqDef:
-      forall bk r H M x ck xs ce,
-        sem_var bk H x xs ->
-        sem_caexp bk H ck ce xs ->
-        msem_equation G bk r H M (EqDef x ck ce)
-  | SEqApp:
-      forall bk r H M x xs ck f M' arg ls xss,
-        Some x = hd_error xs ->
-        mfind_inst x M = Some M' ->
-        sem_laexps bk H ck arg ls ->
-        sem_vars bk H xs xss ->
-        msem_node G r f ls M' xss ->
-        msem_equation G bk r H M (EqApp xs ck f arg None)
-  | SEqReset:
-      forall bk r H M x xs ck f M' arg y ys ls xss,
-        Some x = hd_error xs ->
-        mfind_inst x M = Some M' ->
-        sem_laexps bk H ck arg ls ->
-        sem_vars bk H xs xss ->
-        sem_var bk H y ys ->
-        msem_node G (merge_reset r (reset_of ys)) f ls M' xss ->
-        msem_equation G bk r H M (EqApp xs ck f arg (Some y))
-  (* =msem_equation:fby= *)
-  | SEqFby:
-      forall bk r H M ms x ck ls xs c0 le,
-        mfind_mem x M = Some ms ->
-        ms 0 = sem_const c0 ->
-        sem_laexp bk H ck le ls ->
-        sem_var bk H x xs ->
-        mfby r ls ms xs ->
-        msem_equation G bk r H M (EqFby x ck c0 le)
-  (* =end= *)
+  Section NodeSemantics.
 
-  with msem_node G :
-         stream bool -> ident -> stream (list value) -> memory -> stream (list value) -> Prop :=
-       | SNode:
-           forall bk r f xss M ys i o v eqs ingt0 outgt0 vout defd nodup good,
-             clock_of xss bk ->
-             find_node f G = Some (mk_node f i o v eqs
-                                           ingt0 outgt0 vout defd nodup good) ->
-             (exists H,
-                 sem_vars bk H (map fst i) xss
-                 /\ sem_vars bk H (map fst o) ys
-                 /\ same_clock xss
-                 /\ same_clock ys
-                 /\ (forall n, absent_list (xss n) <-> absent_list (ys n))
-                 /\ Forall (msem_equation G bk r H M) eqs) ->
-             msem_node G r f xss M ys.
+    Variable G: global.
 
-  Definition msem_equations G bk r H M eqs := Forall (msem_equation G bk r H M) eqs.
+    Inductive msem_equation: stream bool -> history -> memory -> equation -> Prop :=
+    | SEqDef:
+        forall bk H M x ck xs ce,
+          sem_var bk H x xs ->
+          sem_caexp bk H ck ce xs ->
+          msem_equation bk H M (EqDef x ck ce)
+    | SEqApp:
+        forall bk H M x xs ck f M' arg ls xss,
+          Some x = hd_error xs ->
+          mfind_inst x M = Some M' ->
+          sem_laexps bk H ck arg ls ->
+          sem_vars bk H xs xss ->
+          msem_node f ls M' xss ->
+          msem_equation bk H M (EqApp xs ck f arg None)
+    | SEqReset:
+        forall bk H M x xs ck f M' arg y ys ls xss,
+          Some x = hd_error xs ->
+          mfind_inst x M = Some M' ->
+          sem_laexps bk H ck arg ls ->
+          sem_vars bk H xs xss ->
+          sem_var bk H y ys ->
+          msem_reset f (reset_of ys) ls M' xss ->
+          msem_equation bk H M (EqApp xs ck f arg (Some y))
+    | SEqFby:
+        forall bk H M ms x ck ls xs c0 le,
+          mfind_mem x M = Some ms ->
+          ms 0 = sem_const c0 ->
+          sem_laexp bk H ck le ls ->
+          sem_var bk H x xs ->
+          mfby ls ms xs ->
+          msem_equation bk H M (EqFby x ck c0 le)
+
+    with msem_reset: ident -> stream bool -> stream (list value) -> memory -> stream (list value) -> Prop :=
+         | SReset:
+             forall f r xss M yss,
+               (forall n, msem_node f (mask (all_absent (xss 0)) n r xss) M
+                               (mask (all_absent (yss 0)) n r yss)) ->
+               msem_reset f r xss M yss
+
+    with msem_node:
+           ident -> stream (list value) -> memory -> stream (list value) -> Prop :=
+         | SNode:
+             forall bk H f xss M yss n,
+               clock_of xss bk ->
+               find_node f G = Some n ->
+               sem_vars bk H (map fst n.(n_in)) xss ->
+               sem_vars bk H (map fst n.(n_out)) yss ->
+               same_clock xss ->
+               same_clock yss ->
+               (forall n, absent_list (xss n) <-> absent_list (yss n)) ->
+               Forall (msem_equation bk H M) n.(n_eqs) ->
+               msem_node f xss M yss.
+
+    Definition msem_equations bk H M eqs := Forall (msem_equation bk H M) eqs.
+
+  End NodeSemantics.
 
   (** ** Induction principle for [msem_equation] and [msem_node] *)
 
@@ -132,264 +146,166 @@ enough: it does not support the internal fixpoint introduced by
 [Forall] *)
 
   Section msem_node_mult.
+
     Variable G: global.
 
-    Variable Pn: forall r (f : ident) xss (M : memory) ys,
-        msem_node G r f xss M ys -> Prop.
-    Variable P: forall bk r (H : history) (M : memory) (eq : equation),
-        msem_equation G bk r H M eq -> Prop.
+    Variable P_equation: stream bool -> history -> memory -> equation -> Prop.
+    Variable P_reset: ident -> stream bool -> stream (list value) -> memory -> stream (list value) -> Prop.
+    Variable P_node: ident -> stream (list value) -> memory -> stream (list value) -> Prop.
 
-    Hypothesis EqDef_case:
-      forall (bk   : stream bool)
-        (r    : stream bool)
-        (H    : history)
-        (M    : memory)
-        (x    : ident)
-        (ck   : clock)
-        (xs   : stream value)
-        (ce   : cexp)
-        (Hvar : sem_var bk H x xs)
-        (Hexp : sem_caexp bk H ck ce xs),
-        P (SEqDef G r M Hvar Hexp).
+    Hypothesis EqDefCase:
+      forall bk H M x ck xs ce,
+        sem_var bk H x xs ->
+        sem_caexp bk H ck ce xs ->
+        P_equation bk H M (EqDef x ck ce).
 
-    Hypothesis EqApp_case:
-      forall (bk     : stream bool)
-        (r      : stream bool)
-        (H      : history)
-        (M      : memory)
-        (x      : ident)
-        (xs     : idents)
-        (ck     : clock)
-        (f      : ident)
-        (M'     : memory)
-        (les    : list lexp)
-        (ls     : stream (list value))
-        (xss    : stream (list value))
-        (Hsome  : Some x = hd_error xs)
-        (Hmfind : mfind_inst x M = Some M')
-        (Hls    : sem_laexps bk H ck les ls)
-        (Hvars  : sem_vars bk H xs xss)
-        (Hmsem  : msem_node G r f ls M' xss),
-        Pn Hmsem
-        -> P (SEqApp M Hsome Hmfind Hls Hvars Hmsem).
+    Hypothesis EqAppCase:
+      forall bk H M x xs ck f M' arg ls xss,
+        Some x = hd_error xs ->
+        mfind_inst x M = Some M' ->
+        sem_laexps bk H ck arg ls ->
+        sem_vars bk H xs xss ->
+        msem_node G f ls M' xss ->
+        P_node f ls M' xss ->
+        P_equation bk H M (EqApp xs ck f arg None).
 
-   Hypothesis EqReset_case:
-      forall (bk     : stream bool)
-        (r      : stream bool)
-        (H      : history)
-        (M      : memory)
-        (x      : ident)
-        (xs     : idents)
-        (ck     : clock)
-        (f      : ident)
-        (M'     : memory)
-        (les    : list lexp)
-        (y      : ident)
-        (ys     : stream value)
-        (ls     : stream (list value))
-        (xss    : stream (list value))
-        (Hsome  : Some x = hd_error xs)
-        (Hmfind : mfind_inst x M = Some M')
-        (Hls    : sem_laexps bk H ck les ls)
-        (Hvars  : sem_vars bk H xs xss)
-        (Hvar   : sem_var bk H y ys)
-        (Hmsem  : msem_node G (merge_reset r (reset_of ys)) f ls M' xss),
-        Pn Hmsem
-        -> P (SEqReset M Hsome Hmfind Hls Hvars Hvar Hmsem).
+    Hypothesis EqResetCase:
+      forall bk H M x xs ck f M' arg y ys ls xss,
+        Some x = hd_error xs ->
+        mfind_inst x M = Some M' ->
+        sem_laexps bk H ck arg ls ->
+        sem_vars bk H xs xss ->
+        sem_var bk H y ys ->
+        msem_reset G f (reset_of ys) ls M' xss ->
+        P_reset f (reset_of ys) ls M' xss ->
+        P_equation bk H M (EqApp xs ck f arg (Some y)).
 
-    Hypothesis EqFby_case:
-      forall (bk     : stream bool)
-        (r      : stream bool)
-        (H      : history)
-        (M      : memory)
-        (ms     : stream val)
-        (y      : ident)
-        (ck     : clock)
-        (ls     : stream value)
-        (yS     : stream value)
-        (c0     : const)
-        (le     : lexp)
-        (Hmfind : mfind_mem y M = Some ms)
-        (Hms0   : ms 0 = sem_const c0)
-        (Hls    : sem_laexp bk H ck le ls)
-        (HyS    : sem_var bk H y yS)
-        (Hy     : mfby r ls ms yS),
-        P (SEqFby G M Hmfind Hms0 Hls HyS Hy).
+    Hypothesis EqFbyCase:
+      forall bk H M ms x ck ls xs c0 le,
+        mfind_mem x M = Some ms ->
+        ms 0 = sem_const c0 ->
+        sem_laexp bk H ck le ls ->
+        sem_var bk H x xs ->
+        mfby ls ms xs ->
+        P_equation bk H M (EqFby x ck c0 le).
 
-    Hypothesis SNode_case:
-      forall (bk     : stream bool)
-        (r      : stream bool)
-        (f      : ident)
-        (xss    : stream (list value))
-        (M      : memory)
-        (yss    : stream (list value))
-        (i      : list (ident * (type * clock)))
-        (o      : list (ident * (type * clock)))
-        (v      : list (ident * (type * clock)))
-        (eqs    : list equation)
-        (ingt0  : 0 < length i)
-        (outgt0 : 0 < length o)
-        (defd   : Permutation (vars_defined eqs)
-                              (map fst (v ++ o)))
-        (vout   : forall x, In x (map fst o) -> ~In x (vars_defined (filter is_fby eqs)))
-        (nodup  : NoDupMembers (i ++ v ++ o))
-        (good   : Forall ValidId (i ++ v ++ o)
-                  /\ Forall valid (vars_defined (filter is_app eqs))
-                  /\ valid f)
-        (Hbk    : clock_of xss bk)
-        (Hfind  : find_node f G =
-                  Some (mk_node f i o v eqs
-                                ingt0 outgt0 defd vout nodup good))
-        (Hnode  : exists H : history,
-            sem_vars bk H (map fst i) xss
-            /\ sem_vars bk H (map fst o) yss
-            /\ same_clock xss
-            /\ same_clock yss
-            /\ (forall n, absent_list (xss n) <-> absent_list (yss n))
-            /\ Forall (msem_equation G bk r H M) eqs),
-        (exists H : history,
-            sem_vars bk H (map fst i) xss
-            /\ sem_vars bk H (map fst o) yss
-            /\ same_clock xss
-            /\ same_clock yss
-            /\ (forall n, absent_list (xss n) <-> absent_list (yss n))
-            /\ Forall (fun eq=>exists Hsem, P (bk := bk) (r := r) (eq := eq)(M := M)(H := H) Hsem) eqs)
-        -> Pn (SNode Hbk Hfind Hnode).
+    Hypothesis ResetCase:
+      forall f r xss M yss,
+        (forall n, msem_node G f (mask (all_absent (xss 0)) n r xss) M (mask (all_absent (yss 0)) n r yss)) ->
+        (forall n, P_node f (mask (all_absent (xss 0)) n r xss) M (mask (all_absent (yss 0)) n r yss)) ->
+        P_reset f r xss M yss.
 
-    Fixpoint msem_node_mult
-             (r   : stream bool)
-             (f   : ident)
-             (xss : stream (list value))
-             (M   : memory)
-             (yss : stream (list value))
-             (Hn  : msem_node G r f xss M yss) {struct Hn}
-      : Pn Hn :=
-      match Hn in (msem_node _ r f xs M ys) return (Pn Hn) with
-      | SNode bk r f xs M ys i o v eqs
-              ingt0 outgt0 defd vout nodup good Hbk Hf Hnode =>
-        SNode_case Hbk Hf Hnode
-                   (* Turn: exists H : history,
-                      (forall n, sem_var H (v_name i) n (xs n))
-                   /\ (forall n, sem_var H (v_name o) n (ys n))
-                   /\ (forall n, xs n = absent
-                                 -> Forall (rhs_absent H n) eqs)
-                   /\ (forall n, xs n = absent <-> ys n = absent)
-                   /\ Forall (msem_equation G H M) eqs
-           Into: exists H : history,
-                      (forall n, sem_var H (v_name i) n (xs n))
-                   /\ (forall n, sem_var H (v_name o) n (ys n))
-                   /\ (forall n, xs n = absent
-                                 -> Forall (rhs_absent H n) eqs)
-                   /\ (forall n, xs n = absent <-> ys n = absent)
-                   /\ Forall (fun eq=>exists Hsem, P H M eq Hsem) eqs *)
-                   (match Hnode with
-                    | ex_intro H (conj Hxs
-                                   (conj Hys
-                                     (conj Hout
-                                       (conj Hsamexs
-                                         (conj Hsameys Heqs))))) =>
-                      ex_intro _ H (conj Hxs (conj Hys (conj Hout
-                                     (conj Hsamexs (conj Hsameys
-                         (((fix map (eqs : list equation)
-                                (Heqs: Forall (msem_equation G bk r H M) eqs) :=
-                              match Heqs in Forall _ fs
-                                    return (Forall (fun eq=> exists Hsem,
-                                                        P Hsem) fs)
-                              with
-                              | Forall_nil => Forall_nil _
-                              | Forall_cons eq eqs Heq Heqs' =>
-                                Forall_cons eq (@ex_intro _ _ Heq
-                                                          (msem_equation_mult Heq))
-                                            (map eqs Heqs')
-                              end) eqs Heqs)))))))
-                    end)
-      end
+    Hypothesis NodeCase:
+      forall bk H f xss M yss n,
+        clock_of xss bk ->
+        find_node f G = Some n ->
+        sem_vars bk H (map fst n.(n_in)) xss ->
+        sem_vars bk H (map fst n.(n_out)) yss ->
+        same_clock xss ->
+        same_clock yss ->
+        (forall n, absent_list (xss n) <-> absent_list (yss n)) ->
+        Forall (msem_equation G bk H M) n.(n_eqs) ->
+        Forall (P_equation bk H M) n.(n_eqs) ->
+        P_node f xss M yss.
 
-    with msem_equation_mult
-           (bk  : stream bool)
-           (r   : stream bool)
-           (H   : history)
-           (M   : memory)
-           (eq  : equation)
-           (Heq : msem_equation G bk r H M eq) {struct Heq}
-         : P Heq :=
-           match Heq in (msem_equation _ _ r H M eq) return (P Heq)
-           with
-           | SEqDef bk r H M y ck xs cae Hvar Hexp => EqDef_case r M Hvar Hexp
-           | SEqApp bk r H M x xs ck f M' lae ls xss Hsome Hmfind Hls Hvars Hmsem =>
-             EqApp_case M Hsome Hmfind Hls Hvars (msem_node_mult Hmsem)
-           | SEqReset bk r H M x xs ck f M' lae y ys ls xss Hsome Hmfind Hls Hvars Hvar Hmsem =>
-             EqReset_case M Hsome Hmfind Hls Hvars Hvar (msem_node_mult Hmsem)
-           | SEqFby bk r H M ms x ck ls yS v0 lae Hmfind Hms0 Hls hyS Hy =>
-  	         EqFby_case M Hmfind Hms0 Hls hyS Hy
-           end.
+    Fixpoint msem_equation_mult
+             (b: stream bool) (H: history) (M: memory) (e: equation)
+             (Sem: msem_equation G b H M e) {struct Sem}
+      : P_equation b H M e
+    with msem_reset_mult
+           (f: ident) (r: stream bool)
+           (xss: stream (list value))
+           (M: memory)
+           (oss: stream (list value))
+           (Sem: msem_reset G f r xss M oss) {struct Sem}
+         : P_reset f r xss M oss
+    with msem_node_mult
+           (f: ident)
+           (xss: stream (list value))
+           (M: memory)
+           (oss: stream (list value))
+           (Sem: msem_node G f xss M oss) {struct Sem}
+         : P_node f xss M oss.
+    Proof.
+      - destruct Sem; eauto.
+      - destruct Sem; eauto.
+      - destruct Sem; eauto.
+        eapply NodeCase; eauto.
+        (* clear H1 defd vout good. *)
+        induction H7; auto.
+    Qed.
+
+    Combined Scheme msem_equation_node_ind from msem_equation_mult, msem_node_mult, msem_reset_mult.
 
   End msem_node_mult.
 
   Definition msem_nodes (G: global) : Prop :=
-    Forall (fun no => exists xs M ys, msem_node G sfalse no.(n_name) xs M ys) G.
-
+    Forall (fun no => exists xs M ys, msem_node G no.(n_name) xs M ys) G.
 
   (** ** Properties *)
 
   (** *** Equation non-activation *)
 
-  Lemma subrate_property_eqn:
-    forall G H M bk r xss eqn n,
-      clock_of xss bk ->
-      msem_equation G bk r H M eqn ->
-      0 < length (xss n) ->
-      absent_list (xss n) ->
-      rhs_absent_instant (bk n) (restr H n) eqn.
-  Proof.
-    intros * Hck Hsem Hlen Habs.
-    assert (Hbk: bk n = false).
-    {
-      destruct (Bool.bool_dec (bk n) false) as [Hbk | Hbk]; eauto.
-      exfalso.
-      apply Bool.not_false_is_true in Hbk.
-      eapply Hck in Hbk.
-      eapply not_absent_present_list in Hbk; auto.
-    }
-    rewrite Hbk in *.
-    destruct eqn;
-      try repeat
-          match goal with
-          | |- rhs_absent_instant false _ (EqDef _ _ _) =>
-            constructor
-          | |- rhs_absent_instant false _ (EqFby _ _ _ _) =>
-            constructor
-          | |- sem_caexp_instant false _ ?ck ?ce absent =>
-            apply SCabs
-          | |- sem_clock_instant false _ ?ck false =>
-            apply subrate_clock
-          | |- sem_laexp_instant false _ ?ck ?le absent =>
-            apply SLabs
-          | |- sem_laexps_instant false _ ?ck ?les _ =>
-            apply SLabss; eauto
-          end.
-    clear Hsem Habs.
-    apply AEqApp with (vs:=map (fun _ =>absent) l).
-    apply SLabss; auto. apply subrate_clock.
-    induction l; [constructor|].
-    apply Forall_cons; auto.
-  Qed.
+  (* Lemma subrate_property_eqn: *)
+  (*   forall G H M bk xss eqn n, *)
+  (*     clock_of xss bk -> *)
+  (*     msem_equation G bk H M eqn -> *)
+  (*     0 < length (xss n) -> *)
+  (*     absent_list (xss n) -> *)
+  (*     rhs_absent_instant (bk n) (restr H n) eqn. *)
+  (* Proof. *)
+  (*   intros * Hck Hsem Hlen Habs. *)
+  (*   assert (Hbk: bk n = false). *)
+  (*   { *)
+  (*     destruct (Bool.bool_dec (bk n) false) as [Hbk | Hbk]; eauto. *)
+  (*     exfalso. *)
+  (*     apply Bool.not_false_is_true in Hbk. *)
+  (*     eapply Hck in Hbk. *)
+  (*     eapply not_absent_present_list in Hbk; auto. *)
+  (*   } *)
+  (*   rewrite Hbk in *. *)
+  (*   destruct eqn. *)
+  (*   constructor. *)
+  (*   apply SCabs; try apply subrate_clock. *)
 
-  Lemma subrate_property_eqns:
-    forall G H M bk r xss eqns n,
-      clock_of xss bk ->
-      msem_equations G bk r H M eqns ->
-      0 < length (xss n) ->
-      absent_list (xss n) ->
-      Forall (rhs_absent_instant (bk n) (restr H n)) eqns.
-  Proof.
-    intros * Hck Hsem Habs.
-    induction eqns as [|eqn eqns]; auto.
-    inversion_clear Hsem.
-    constructor.
-    eapply subrate_property_eqn; eauto.
-    eapply IHeqns; eauto.
-  Qed.
+  (*   ; *)
+  (*     try repeat *)
+  (*         match goal with *)
+  (*         | |- rhs_absent_instant false _ (EqDef _ _ _) => *)
+  (*           constructor *)
+  (*         | |- rhs_absent_instant false _ (EqFby _ _ _ _) => *)
+  (*           constructor *)
+  (*         | |- sem_caexp_instant false _ ?ck ?ce absent => *)
+  (*           apply SCabs *)
+  (*         | |- sem_clock_instant false _ ?ck false => *)
+  (*           apply subrate_clock *)
+  (*         | |- sem_laexp_instant false _ ?ck ?le absent => *)
+  (*           apply SLabs *)
+  (*         | |- sem_laexps_instant false _ ?ck ?les _ => *)
+  (*           apply SLabss; eauto *)
+  (*         end. *)
+  (*   clear Hsem Habs. *)
+  (*   apply AEqApp with (vs:=map (fun _ =>absent) l). *)
+  (*   apply SLabss; auto. apply subrate_clock. *)
+  (*   induction l; [constructor|]. *)
+  (*   apply Forall_cons; auto. *)
+  (* Qed. *)
+
+  (* Lemma subrate_property_eqns: *)
+  (*   forall G H M bk xss eqns n, *)
+  (*     clock_of xss bk -> *)
+  (*     msem_equations G bk H M eqns -> *)
+  (*     0 < length (xss n) -> *)
+  (*     absent_list (xss n) -> *)
+  (*     Forall (rhs_absent_instant (bk n) (restr H n)) eqns. *)
+  (* Proof. *)
+  (*   intros * Hck Hsem Habs. *)
+  (*   induction eqns as [|eqn eqns]; auto. *)
+  (*   inversion_clear Hsem. *)
+  (*   constructor. *)
+  (*   eapply subrate_property_eqn; eauto. *)
+  (*   eapply IHeqns; eauto. *)
+  (* Qed. *)
 
   (** *** Environment cons-ing lemmas *)
 
@@ -401,117 +317,107 @@ enough: it does not support the internal fixpoint introduced by
    TODO: try this when the other elements are stabilised. *)
 
   Lemma msem_node_cons:
-    forall node G r f xs M ys,
-      Ordered_nodes (node::G)
-      -> msem_node (node :: G) r f xs M ys
-      -> node.(n_name) <> f
-      -> msem_node G r f xs M ys.
+    forall n G f xs M ys,
+      Ordered_nodes (n :: G) ->
+      msem_node (n :: G) f xs M ys ->
+      n.(n_name) <> f ->
+      msem_node G f xs M ys.
   Proof.
-    intros node G r f xs M ys Hord Hsem Hnf.
+    Hint Constructors msem_equation msem_reset.
+    intros ** Hord Hsem Hnf.
     revert Hnf.
-    induction Hsem as [
-        | bk r H M x xs ck f M' les ls xss Hsome Hmfind Hls Hvars Hmsem IH
-        | bk r H M x xs ck f M' les y ys ls xss Hsome Hmfind Hls Hvars Hvar Hmsem IH
-        |
-        | bk r f xs M ys i o v eqs ingt0 outgt0 defd vout nodup good Hbk Hf Heqs IH ]
+    induction Hsem as [| | | | | ? ? ? ? ? ? ? ? Hf ? ? ? ? ? ? IH ]
         using msem_node_mult
-        with (P := fun bk r H M eq Hsem => ~Is_node_in_eq node.(n_name) eq
-                                         -> msem_equation G bk r H M eq).
-    - econstructor; eauto.
+      with (P_equation := fun bk H M eq =>
+                            ~Is_node_in_eq n.(n_name) eq ->
+                            msem_equation G bk H M eq)
+           (P_reset := fun f bk xss M yss =>
+                         n_name n <> f ->
+                         msem_reset G f bk xss M yss); eauto.
     - intro Hnin.
-      assert (msem_node G r f ls M' xss).
-      {
-        apply IH. intro Hnf. apply Hnin. rewrite Hnf. constructor.
-      }
-
-      eapply SEqApp; eauto.
+      econstructor; eauto.
+      apply IHHsem. intro Hnf; apply Hnin; rewrite Hnf. constructor.
     - intro Hnin.
-      assert (msem_node G (merge_reset r (reset_of ys)) f ls M' xss).
-      {
-        apply IH. intro Hnf. apply Hnin. rewrite Hnf. constructor.
-      }
-
-      eapply SEqReset; eauto.
-    - intro; eapply SEqFby; eassumption.
+      econstructor; eauto.
+      apply IHHsem. intro Hnf; apply Hnin; rewrite Hnf. constructor.
     - intro.
       rewrite find_node_tl with (1:=Hnf) in Hf.
-      eapply SNode; eauto.
-      clear Heqs.
-      destruct IH as (H & Hxs & Hys & Hout & Hsamexs & Hsameys & Heqs).
-      exists H.
-      repeat (split; auto).
+      econstructor; eauto.
       apply find_node_later_not_Is_node_in with (2:=Hf) in Hord.
       apply Is_node_in_Forall in Hord.
-      apply Forall_Forall with (1:=Hord) in Heqs.
-      apply Forall_impl with (2:=Heqs).
-      destruct 1 as [Hnini [Hsem HH]].
+      apply Forall_Forall with (1:=Hord) in IH.
+      apply Forall_impl with (2:=IH).
       intuition.
   Qed.
 
+  Corollary msem_reset_cons:
+    forall n G f bk xs M ys,
+      Ordered_nodes (n :: G) ->
+      msem_reset (n :: G) f bk xs M ys ->
+      n.(n_name) <> f ->
+      msem_reset G f bk xs M ys.
+  Proof.
+    intros ** Sem ?.
+    inv Sem.
+    constructor; intro.
+    eauto using msem_node_cons.
+  Qed.
+
   Lemma msem_node_cons2:
-    forall nd G r f xs M ys,
-      Ordered_nodes G
-      -> msem_node G r f xs M ys
-      -> Forall (fun nd' : node => n_name nd <> n_name nd') G
-      -> msem_node (nd::G) r f xs M ys.
+    forall n G f xs M ys,
+      Ordered_nodes G ->
+      msem_node G f xs M ys ->
+      Forall (fun n' => n_name n <> n_name n') G ->
+      msem_node (n :: G) f xs M ys.
   Proof.
     Hint Constructors msem_equation.
-    intros nd G r f xs M ys Hord Hsem Hnin.
+    intros ** Hord Hsem Hnin.
     assert (Hnin':=Hnin).
     revert Hnin'.
-    induction Hsem as [
-        | bk r H M x xs ck f M' les ls xss Hsome Hmfind Hls Hvars Hmsem IH
-        | bk r H M x xs ck f M' les y ys ls xss Hsome Hmfind Hls Hvars Hvar Hmsem IH
-        |
-        | bk r f xs M ys i o v eqs
-             ingt0 outgt0 defd vout nodup good Hbk Hfind Heqs IH ]
+    induction Hsem as [| | | | | ? ? ? ? ? ? n' ? Hfind ? ? ? ? ? Heqs IH ]
         using msem_node_mult
-        with (P := fun bk r H M eq Hsem => ~Is_node_in_eq nd.(n_name) eq
-                                         -> msem_equation (nd::G) bk r H M eq);
-      try eauto; intro HH.
-    clear HH.
-    assert (nd.(n_name) <> f) as Hnf.
+      with (P_equation := fun bk H M eq =>
+                            ~Is_node_in_eq n.(n_name) eq ->
+                            msem_equation (n :: G) bk H M eq)
+           (P_reset := fun f bk xss M yss =>
+                         Forall (fun n' : node => n_name n <> n_name n') G ->
+                         msem_reset (n :: G) f bk xss M yss); eauto.
+    intro HH; clear HH.
+    assert (n.(n_name) <> f) as Hnf.
     { intro Hnf.
       rewrite Hnf in *.
+      pose proof (find_node_name _ _ _ Hfind).
       apply find_node_split in Hfind.
       destruct Hfind as [bG [aG Hge]].
       rewrite Hge in Hnin.
       apply Forall_app in Hnin.
-      destruct Hnin as [H0 Hfg]; clear H0.
+      destruct Hnin as [H' Hfg]; clear H'.
       inversion_clear Hfg.
-      match goal with H:f<>_ |- False => apply H end.
-      reflexivity. }
+      match goal with H:f<>_ |- False => now apply H end.
+    }
     apply find_node_other with (2:=Hfind) in Hnf.
     econstructor; eauto.
-    clear Heqs.
-    destruct IH as (H & Hxs & Hys & Hout & Hsamexs & Hsameys & Heqs).
-    exists H.
-    intuition; clear Hxs Hys.
-    assert (forall g, Is_node_in g eqs
-                      -> Exists (fun nd=> g = nd.(n_name)) G)
-      as Hniex
-        by (intros g Hini;
-             apply find_node_find_again with (1:=Hord) (2:=Hfind) in Hini;
-             exact Hini).
-    assert (Forall
-              (fun eq=> forall g,
-                   Is_node_in_eq g eq
-                   -> Exists (fun nd=> g = nd.(n_name)) G) eqs) as HH.
+    assert (forall g, Is_node_in g n'.(n_eqs) -> Exists (fun nd=> g = nd.(n_name)) G)
+      as Hniex by (intros g Hini;
+                   apply find_node_find_again with (1:=Hord) (2:=Hfind) in Hini;
+                   exact Hini).
+    assert (Forall (fun eq => forall g,
+                        Is_node_in_eq g eq -> Exists (fun nd=> g = nd.(n_name)) G)
+                   n'.(n_eqs)) as HH.
     {
-      clear defd vout nodup good Hfind Heqs Hnf.
-      induction eqs as [|eq eqs IH]; [now constructor|].
+      clear Heqs IH.
+      induction n'.(n_eqs) as [|eq eqs]; [now constructor|].
       constructor.
       - intros g Hini.
         apply Hniex.
         constructor 1; apply Hini.
-      - apply IH.
+      - apply IHeqs.
         intros g Hini; apply Hniex.
         constructor 2; apply Hini.
     }
-    apply Forall_Forall with (1:=HH) in Heqs.
-    apply Forall_impl with (2:=Heqs).
-    intros eq IH.
-    destruct IH as [Hsem [IH0 IH1]].
+    apply Forall_Forall with (1:=HH) in IH.
+    apply Forall_impl with (2:=IH).
+    intros eq (Hsem & IH1).
     apply IH1.
     intro Hini.
     apply Hsem in Hini.
@@ -521,15 +427,28 @@ enough: it does not support the internal fixpoint introduced by
     intuition.
   Qed.
 
+  Lemma msem_reset_cons2:
+    forall n G f bk xs M ys,
+      Ordered_nodes G ->
+      msem_reset G f bk xs M ys ->
+      Forall (fun n' => n_name n <> n_name n') G ->
+      msem_reset (n :: G) f bk xs M ys.
+  Proof.
+    intros ** Sem ?.
+    inv Sem.
+    constructor; intro.
+    eauto using msem_node_cons2.
+  Qed.
+
   Lemma msem_equation_cons2:
-    forall G bk r H M eqs nd,
-      Ordered_nodes (nd::G)
-      -> Forall (msem_equation G bk r H M) eqs
-      -> ~Is_node_in nd.(n_name) eqs
-      -> Forall (msem_equation (nd::G) bk r H M) eqs.
+    forall G bk H M eqs n,
+      Ordered_nodes (n :: G) ->
+      Forall (msem_equation G bk H M) eqs ->
+      ~Is_node_in n.(n_name) eqs ->
+      Forall (msem_equation (n :: G) bk H M) eqs.
   Proof.
     Hint Constructors msem_equation.
-    intros G bk r H M eqs nd Hord Hsem Hnini.
+    intros ** Hord Hsem Hnini.
     induction eqs as [|eq eqs IH]; [now constructor|].
     apply Forall_cons2 in Hsem.
     destruct Hsem as [Heq Heqs].
@@ -537,24 +456,19 @@ enough: it does not support the internal fixpoint introduced by
     destruct Hnini as [Hnini Hninis].
     apply IH with (2:=Hninis) in Heqs.
     constructor; [|now apply Heqs].
-    destruct Heq as [|? ? ? ? ? ? ? ? ? ? ? ? Hsome Hmfind Hls Hvars Hmsem
-                        |? ? ? ? ? ? ? ? ? ? ? ? ? ? Hsome Hmfind Hls Hvars Hvar Hmsem|];
+    inv Hord.
+    destruct Heq as [| |? ? ? ? ? ? ? ? ? ? ? ? ? ? ? ? ? ? Hmsem|];
       try now eauto.
-    - econstructor; eauto.
-      inversion_clear Hord as [|? ? Hord' Hnn Hnns].
-      apply msem_node_cons2 with (1:=Hord') (3:=Hnns).
-      apply Hmsem.
-    - econstructor; eauto.
-      inversion_clear Hord as [|? ? Hord' Hnn Hnns].
-      apply msem_node_cons2 with (1:=Hord') (3:=Hnns).
-      apply Hmsem.
+    - eauto using msem_node_cons2.
+    - eauto using msem_reset_cons2.
   Qed.
 
   Lemma find_node_msem_node:
     forall G f,
-      msem_nodes G
-      -> find_node f G <> None
-      -> (exists xs M ys, msem_node G sfalse f xs M ys).
+      msem_nodes G ->
+      find_node f G <> None ->
+      exists xs M ys,
+        msem_node G f xs M ys.
   Proof.
     intros G f Hnds Hfind.
     apply find_node_Exists in Hfind.
@@ -569,17 +483,16 @@ enough: it does not support the internal fixpoint introduced by
     exact Hmsem.
   Qed.
 
-
   (* TODO: Tidy this up... *)
   Lemma Forall_msem_equation_global_tl:
-    forall nd G bk r H M eqs,
-      Ordered_nodes (nd::G)
-      -> (forall f, Is_node_in f eqs -> find_node f G <> None)
-      -> ~ Is_node_in nd.(n_name) eqs
-      -> Forall (msem_equation (nd::G) bk r H M) eqs
-      -> Forall (msem_equation G bk r H M) eqs.
+    forall n G bk H M eqs,
+      Ordered_nodes (n :: G) ->
+      (forall f, Is_node_in f eqs -> find_node f G <> None) ->
+      ~ Is_node_in n.(n_name) eqs ->
+      Forall (msem_equation (n :: G) bk H M) eqs ->
+      Forall (msem_equation G bk H M) eqs.
   Proof.
-    intros nd G bk r H M eqs Hord.
+    intros ? ? ? ? ? ? Hord.
     induction eqs as [|eq eqs IH]; trivial; [].
     intros Hfind Hnini Hmsem.
     apply Forall_cons2 in Hmsem; destruct Hmsem as [Hseq Hseqs].
@@ -587,19 +500,11 @@ enough: it does not support the internal fixpoint introduced by
     - apply Forall_cons; trivial.
       apply not_Is_node_in_cons in Hnini.
       destruct Hnini.
-      inv Hseq; eauto.
-      + assert (nd.(n_name) <> f).
-        { intro HH.
-          apply H0.
-          rewrite HH.
-          constructor. }
-        eauto using msem_node_cons.
-      +  assert (nd.(n_name) <> f).
-        { intro HH.
-          apply H0.
-          rewrite HH.
-          constructor. }
-        eauto using msem_node_cons.
+      inv Hseq; eauto;
+        assert (n.(n_name) <> f)
+        by (intro HH; apply H0; rewrite HH; constructor).
+      + eauto using msem_node_cons.
+      + eauto using msem_reset_cons.
     - intros f Hini.
       apply (Exists_cons_tl eq) in Hini.
       now apply (Hfind _ Hini).
@@ -610,32 +515,31 @@ enough: it does not support the internal fixpoint introduced by
   (** *** Memory management *)
 
   Lemma msem_equation_madd_mem:
-    forall G bk r H M x ms eqs,
-      ~Is_defined_in_eqs x eqs
-      -> Forall (msem_equation G bk r H M) eqs
-      -> Forall (msem_equation G bk r H (madd_mem x ms M)) eqs.
+    forall G bk H M x ms eqs,
+      ~Is_defined_in_eqs x eqs ->
+      Forall (msem_equation G bk H M) eqs ->
+      Forall (msem_equation G bk H (madd_mem x ms M)) eqs.
   Proof.
     Hint Constructors msem_equation.
-    intros G bk r H M x ms eqs Hnd Hsem.
+    intros ** Hnd Hsem.
     induction eqs as [|eq eqs IH]; [now constructor|].
     apply not_Is_defined_in_cons in Hnd.
     destruct Hnd as [Hnd Hnds].
     apply Forall_cons2 in Hsem.
     destruct Hsem as [Hsem Hsems].
     constructor; [|now apply IH with (1:=Hnds) (2:=Hsems)].
-    destruct Hsem as [| | |? ? ? ? ? ? ? ? ? ? ? Hmfind]; try now eauto.
+    destruct Hsem; eauto.
     apply not_Is_defined_in_eq_EqFby in Hnd.
     eapply SEqFby; try eassumption.
     apply not_eq_sym in Hnd.
-    rewrite mfind_mem_gso with (1:=Hnd).
-    exact Hmfind.
+    now rewrite mfind_mem_gso with (1:=Hnd).
   Qed.
 
   Lemma msem_equation_madd_obj:
-    forall G bk r H M M' x eqs,
-      ~Is_defined_in_eqs x eqs
-      -> Forall (msem_equation G bk r H M) eqs
-      -> Forall (msem_equation G bk r H (madd_obj x M' M)) eqs.
+    forall G bk H M M' x eqs,
+      ~Is_defined_in_eqs x eqs ->
+      Forall (msem_equation G bk H M) eqs ->
+      Forall (msem_equation G bk H (madd_obj x M' M)) eqs.
   Proof.
     Hint Constructors msem_equation.
     intros * Hnd Hsem.
@@ -645,27 +549,14 @@ enough: it does not support the internal fixpoint introduced by
     apply Forall_cons2 in Hsem.
     destruct Hsem as [Hsem Hsems].
     constructor; [|now apply IH with (1:=Hnds) (2:=Hsems)].
-    destruct Hsem as [|? ? ? ? ? ? ? ? ? ? ? ? Hsome Hmfind Hls Hvars Hmsem
-                         |? ? ? ? ? ? ? ? ? ? ? ? ? ? Hsome Hmfind Hls Hvars Hvar Hmsem|];
-      try now eauto.
-    - apply not_Is_defined_in_eq_EqApp in Hnd.
-      econstructor; eauto.
-      assert (x0 <> x).
-      {
-        intro; subst x.
-        destruct xs; inv Hsome. apply Hnd. constructor (auto).
-      }
-      erewrite mfind_inst_gso; eauto.
-    - apply not_Is_defined_in_eq_EqApp in Hnd.
-      econstructor; eauto.
-      assert (x0 <> x).
-      {
-        intro; subst x.
-        destruct xs; inv Hsome. apply Hnd. constructor (auto).
-      }
-      erewrite mfind_inst_gso; eauto.
+    destruct Hsem as [|? ? ? x' ? ? ? ? ? ? ? Hsome Hmfind Hls Hvars Hmsem
+                         |? ? ? x' ? ? ? ? ? ? ? ? ? Hsome Hmfind Hls Hvars Hvar Hmsem|];
+      eauto;
+      assert (mfind_inst x' (madd_obj x M' M) = Some M'0)
+        by (apply not_Is_defined_in_eq_EqApp in Hnd;
+            rewrite mfind_inst_gso; auto;
+            intro; subst x; destruct xs; inv Hsome; apply Hnd; now constructor); eauto.
   Qed.
-
 
   (* XXX: I believe that this comment is outdated ([no_dup_defs] is long gone)
 
@@ -709,23 +600,22 @@ dataflow memory for which the non-standard semantics holds true.
    *)
 
   Lemma sem_msem_eq:
-    forall G bk r H eqs M eq mems argIn,
-      (forall r f xs ys,
-          sem_node G r f xs ys
-          -> exists M : memory, msem_node G r f xs M ys)
-      -> sem_equation G bk r H eq
-      -> Is_well_sch mems argIn (eq::eqs)
-      -> Forall (msem_equation G bk r H M) eqs
-      -> exists M', Forall (msem_equation G bk r H M') (eq::eqs).
+    forall G bk H eqs M eq mems argIn,
+      (forall f xs ys,
+          sem_node G f xs ys ->
+          exists M, msem_node G f xs M ys) ->
+      sem_equation G bk H eq ->
+      Is_well_sch mems argIn (eq :: eqs) ->
+      Forall (msem_equation G bk H M) eqs ->
+      exists M', Forall (msem_equation G bk H M') (eq :: eqs).
   Proof.
-    intros G bk r H eqs M eq mems argIn IH Heq Hwsch Hmeqs.
-    inversion Heq as [? ? ? ? ? ? ? Hsem
-                        |? ? ? ? ? ? ? ? ? Hls Hxs Hsem
-                        |? ? ? ? ? ? ? ? ? ? ? Hls Hxs Hy Hsem
-                        |? ? ? ? ? ? ? ? ? Hle Hvar];
+    intros ** IH Heq Hwsch Hmeqs.
+    inversion Heq as [|? ? ? ? ? ? ? ? Hls Hxs Hsem
+                         |? ? ? ? ? ? ? ? ? ? Hls Hxs Hy Hsem
+                         |? ? ? ? ? ? ? ? Hle Hvar];
       match goal with H:_=eq |- _ => rewrite <-H in * end.
     - exists M.
-      constructor ((econstructor; eassumption) || assumption).
+      repeat (econstructor; eauto).
     - apply IH in Hsem.
       destruct Hsem as [M' Hmsem].
       exists (madd_obj (hd Ids.default x) M' M).
@@ -734,32 +624,16 @@ dataflow memory for which the non-standard semantics holds true.
       {
         assert (Hlen: 0 < length x).
         {
-          assert (length x = length (xs 0)).
-          {
-            specialize (Hxs 0); simpl in Hxs.
-            eapply Forall2_length; eauto.
-          }
+          assert (length x = length (xs 0))
+            by (specialize (Hxs 0); simpl in Hxs; eapply Forall2_length; eauto).
 
-          assert (exists n,   length (map fst n.(n_out)) = length (xs 0)
+          assert (exists n, length (map fst n.(n_out)) = length (xs 0)
                        /\ 0 < length n.(n_out)) as (n & ? & ?).
           {
-            destruct Hmsem as [ ? ? ? ? ? ? ? ? ? ? ? ? ? ? ? ? ? ? Hsem].
-            decompose record Hsem.
-            eexists {| n_name := f;
-                       n_in := i;  n_out := o; n_vars := v;
-                       n_eqs := eqs0;
-                       n_ingt0 := ingt0;
-                       n_outgt0 := outgt0;
-                       n_defd := vout;
-                       n_vout := defd;
-                       n_nodup := nodup;
-                       n_good := good |}; simpl.
-            split; auto.
-            match goal with
-            | H: sem_vars _ _ (map fst o) ys |- _ =>
-              specialize (H 0); simpl in H
-            end.
-            eapply Forall2_length; eauto.
+            inv Hmsem.
+            exists n; split; auto.
+            - eapply Forall2_length; eauto.
+            - exact n.(n_outgt0).
           }
 
           assert (length (map fst n.(n_out)) = length n.(n_out))
@@ -776,11 +650,13 @@ dataflow memory for which the non-standard semantics holds true.
       {
         destruct x; simpl in *; try discriminate.
         injection Hsome; congruence.
-      } rewrite Hhd; clear Hhd.
+      }
+
+      rewrite Hhd; clear Hhd.
 
       constructor.
-      econstructor; eauto.
-      + now apply mfind_inst_gss.
+      + econstructor; eauto.
+        now apply mfind_inst_gss.
       + inversion_clear Hwsch.
         assert (Is_defined_in_eq i (EqApp x ck f arg None)).
         {
@@ -789,70 +665,72 @@ dataflow memory for which the non-standard semantics holds true.
         }
         now apply msem_equation_madd_obj; auto.
 
-    - apply IH in Hsem.
-      destruct Hsem as [M' Hmsem].
-      exists (madd_obj (hd Ids.default x) M' M).
+    - admit.
 
-      assert (exists i, Some i = hd_error x) as [i Hsome].
-      {
-        assert (Hlen: 0 < length x).
-        {
-          assert (length x = length (xs 0)).
-          {
-            specialize (Hxs 0); simpl in Hxs.
-            eapply Forall2_length; eauto.
-          }
+      (* inv Hsem. apply IH in Hsem. *)
+      (* destruct Hsem as [M' Hmsem]. *)
+      (* exists (madd_obj (hd Ids.default x) M' M). *)
 
-          assert (exists n,   length (map fst n.(n_out)) = length (xs 0)
-                       /\ 0 < length n.(n_out)) as (n & ? & ?).
-          {
-            destruct Hmsem as [ ? ? ? ? ? ? ? ? ? ? ? ? ? ? ? ? ? ? Hsem].
-            decompose record Hsem.
-            eexists {| n_name := f;
-                       n_in := i;  n_out := o; n_vars := v;
-                       n_eqs := eqs0;
-                       n_ingt0 := ingt0;
-                       n_outgt0 := outgt0;
-                       n_defd := vout;
-                       n_vout := defd;
-                       n_nodup := nodup;
-                       n_good := good |}; simpl.
-            split; auto.
-            match goal with
-            | H: sem_vars _ _ (map fst o) ys0 |- _ =>
-              specialize (H 0); simpl in H
-            end.
-            eapply Forall2_length; eauto.
-          }
+      (* assert (exists i, Some i = hd_error x) as [i Hsome]. *)
+      (* { *)
+      (*   assert (Hlen: 0 < length x). *)
+      (*   { *)
+      (*     assert (length x = length (xs 0)). *)
+      (*     { *)
+      (*       specialize (Hxs 0); simpl in Hxs. *)
+      (*       eapply Forall2_length; eauto. *)
+      (*     } *)
 
-          assert (length (map fst n.(n_out)) = length n.(n_out))
-            by apply map_length.
+      (*     assert (exists n,   length (map fst n.(n_out)) = length (xs 0) *)
+      (*                  /\ 0 < length n.(n_out)) as (n & ? & ?). *)
+      (*     { *)
+      (*       destruct Hmsem as [ ? ? ? ? ? ? ? ? ? ? ? ? ? ? ? ? ? ? Hsem]. *)
+      (*       decompose record Hsem. *)
+      (*       eexists {| n_name := f; *)
+      (*                  n_in := i;  n_out := o; n_vars := v; *)
+      (*                  n_eqs := eqs0; *)
+      (*                  n_ingt0 := ingt0; *)
+      (*                  n_outgt0 := outgt0; *)
+      (*                  n_defd := vout; *)
+      (*                  n_vout := defd; *)
+      (*                  n_nodup := nodup; *)
+      (*                  n_good := good |}; simpl. *)
+      (*       split; auto. *)
+      (*       match goal with *)
+      (*       | H: sem_vars _ _ (map fst o) ys0 |- _ => *)
+      (*         specialize (H 0); simpl in H *)
+      (*       end. *)
+      (*       eapply Forall2_length; eauto. *)
+      (*     } *)
 
-          now congruence.
-        }
+      (*     assert (length (map fst n.(n_out)) = length n.(n_out)) *)
+      (*       by apply map_length. *)
 
-        destruct x; try now inv Hlen.
-        eexists; simpl; eauto.
-      }
+      (*     now congruence. *)
+      (*   } *)
 
-      assert (Hhd: hd Ids.default x = i).
-      {
-        destruct x; simpl in *; try discriminate.
-        injection Hsome; congruence.
-      } rewrite Hhd; clear Hhd.
+      (*   destruct x; try now inv Hlen. *)
+      (*   eexists; simpl; eauto. *)
+      (* } *)
 
-      constructor.
-      econstructor; eauto.
-      + now apply mfind_inst_gss.
-      + inversion_clear Hwsch.
-        assert (Is_defined_in_eq i (EqApp x ck f arg (Some y))).
-        {
-          constructor. destruct x; try discriminate.
-          injection Hsome. intro; subst i. constructor (auto).
-        }
-        apply msem_equation_madd_obj; auto.
+      (* assert (Hhd: hd Ids.default x = i). *)
+      (* { *)
+      (*   destruct x; simpl in *; try discriminate. *)
+      (*   injection Hsome; congruence. *)
+      (* } rewrite Hhd; clear Hhd. *)
 
-    - exists (madd_mem x (hold r (sem_const c0) ls) M).
+      (* constructor. *)
+      (* econstructor; eauto. *)
+      (* + now apply mfind_inst_gss. *)
+      (* + inversion_clear Hwsch. *)
+      (*   assert (Is_defined_in_eq i (EqApp x ck f arg (Some y))). *)
+      (*   { *)
+      (*     constructor. destruct x; try discriminate. *)
+      (*     injection Hsome. intro; subst i. constructor (auto). *)
+      (*   } *)
+      (*   apply msem_equation_madd_obj; auto. *)
+
+    - exists (madd_mem x (hold (sem_const c0) ls) M).
       constructor.
       econstructor; eauto.
       + now apply mfind_mem_gss.
